

Exercise 1.1.1:  $C_n = \begin{cases} \mathbb{Z}_8 & n \geq 0 \\ 0 & n < 0 \end{cases} \quad d_n([x]_8) = [4x]_8 \quad (1)$

$d_{n-1} \circ d_n(x) = 8x \equiv 0$  so it's a chain complex.

$Z_n = \{0, 2, 4, 6\} \quad 0 \mapsto 0, 1 \mapsto 4, 2 \mapsto 0, 3 \mapsto 4$

$4 \mapsto 0, 5 \mapsto 4, 6 \mapsto 0, 7 \mapsto 4$

$B_n = \{0, 4\}$

$$H_n = \begin{cases} \mathbb{Z}_2 & n > 0 \\ \mathbb{Z}_4 & n = 0 \\ 0 & \text{otherwise} \end{cases}$$

$$\begin{array}{ccccccc} \mathbb{Z}_8 & \xrightarrow{4} & \mathbb{Z}_8 & \xrightarrow{4} & \mathbb{Z}_8 & \xrightarrow{4} & \mathbb{Z}_8 \xrightarrow{0} 0 \xrightarrow{0} 0 \\ & \swarrow \langle 2 \rangle / \langle 4 \rangle & \swarrow \langle 2 \rangle / \langle 4 \rangle & \swarrow \mathbb{Z}_8 / \langle 4 \rangle & & & \\ & \mathbb{Z}_2 & \mathbb{Z}_2 & \mathbb{Z}_4 & & 0 & 0 \end{array}$$

Exercise 1.1.2:

$$\begin{array}{ccccccc} \cdots & \longrightarrow & C_{n+1} & \xrightarrow{d_{n+1}} & C_n & \xrightarrow{d_n} & C_{n-1} \longrightarrow \cdots \\ & & \downarrow U_{n+1} & & \downarrow U_n & & \downarrow U_{n-1} \\ \cdots & \longrightarrow & D_{n+1} & \xrightarrow{d_{n+1}} & D_n & \xrightarrow{d_n} & D_{n-1} \longrightarrow \cdots \end{array}$$

Suppose  $b \in B_n^C$ , then  $b = d_{n+1}(c)$  for some  $c \in C_{n+1}$ . So

$$U_n(b) = U_n(d_{n+1}(c)) = d_{n+1} \circ U_{n+1}(c) \in \text{Im}(d_{n+1}) \subseteq B_n^D$$

Thus  $U_n(B_n^C) \subseteq B_n^D$ .

Suppose  $z \in Z_n^C$ . Then  $d_n(z) = 0$  and since  $U_{n-1}$  is a hom. of modules,

$$U_{n-1}(0) = 0, \text{ so } d_n(U_n(z)) = U_{n-1}(d_n(z)) = U_{n-1}(0) = 0$$

So  $U_n(z) \in \ker d_{n-1}$ . Thus,  $U_n(Z_n^C) \subseteq Z_n^D$ .

This means we get an induced map  $H_n(C) \longrightarrow H_n(D)$ .

$H_n$  is a functor: (1)  $\text{id}_C^* : H_n(C) \longrightarrow H_n(C)$ .  $\text{id}_C(z_n) = z_n, \text{id}_C(B_n) = B_n$

$$\Rightarrow \text{Id}_C^*(z + B_n) = z + B_n = \text{Id}_{H_n(C)}(z + B_n), \text{ so } \text{Id}_C^* = \text{Id}_{H_n(C)}.$$

$$(2) (f \circ g)^*(z + B_n) = f \circ g(z) + f \circ g(B_n) = f^*(g(z) + g(B_n)) = f^* \circ g^*(z + B_n)$$

$$\text{so } (f \circ g)^* = f^* \circ g^*$$

Exercise 1.13: Let  $\{B_n, H_n\}$  vec. spaces over a field  $K$ .

Let  $C_n = B_n \oplus H_n \oplus B_{n-1}$ . Define  $\psi_n: C_n \rightarrow C_{n-1}$  by proj. onto third component, then inclusion to the first component of  $C_{n-1}$ .

Clearly each  $C_n$  is a vector space, and each  $H_n$  is a vector space homomorphism. Let  $(b, h, b') \in C_{n+1}$ . Then

$$\psi_n \circ \psi_{n+1}(b, h, b') = \psi_n(b', 0, 0) = (0, 0, 0)$$

So the composite of any two is 0.

Now, suppose  $\{V_n\}$  is a family of  $K$ -vector spaces and

$$\cdots \xrightarrow{d} V_{n+1} \xrightarrow{d} V_n \xrightarrow{d} V_{n-1} \xrightarrow{d} 0$$

is a chain complex. Then for each  $V_n$  we can decompose

$$\text{it as } V_n = \text{Im } d_{n+1} \oplus \text{Ker } d_n / \text{Im } d_{n+1} \oplus V_n / \text{Ker } d_n$$

Since  $V_n / \text{Ker } d_n \cong \text{Im } d_n$  we can choose

$$B_n = \text{Im } d_{n+1}$$

$$H_n = \text{Ker } d_n / \text{Im } d_{n+1}$$

$$\text{So } V_n = B_n \oplus H_n \oplus V_n / \text{Ker } d_n \cong B_n \oplus H_n \oplus \text{Im } d_n = B_n \oplus H_n \oplus B_{n-1}$$

and  $\psi_n$  is proj.-inclusion as claimed.

Exercise 1.14: Let  $\dots \xrightarrow{d} C_{n+1} \rightarrow C_n \rightarrow C_{n-1} \rightarrow \dots$  be a chain complex. Then consider the sequence

$$\dots \rightarrow \text{Hom}_{\mathbb{Z}}(A, C_{n+1}) \rightarrow \text{Hom}_{\mathbb{Z}}(A, C_n) \rightarrow \text{Hom}_{\mathbb{Z}}(A, C_{n-1}) \rightarrow \dots$$

where  $d(f) = d_n \circ f$  for any  $f \in \text{Hom}_{\mathbb{Z}}(A, C_n)$ . These are homomorphisms and  $d_n$  is the same  $d_n$  as in  $C$ .

$$d_n \circ d_{n+1}(f) = d_n(d_{n+1} \circ f) = (d_n \circ d_{n+1}) \circ f = 0 \circ f = 0.$$

So it's a chain complex.

→ Suppose  $A = \mathbb{Z}_n$ , and  $H_n(\text{Hom}_{\mathbb{Z}}(\mathbb{Z}_n, C)) = 0$ .

$$0 = H_n(\text{Hom}_{\mathbb{Z}}(\mathbb{Z}_n, C)) = \text{Ker}(d'_n) / \text{Im}(d'_{n+1}) \iff \text{Ker}(d'_n) = \text{Im}(d'_{n+1})$$

So any map  $f_n \in \text{Hom}_{\mathbb{Z}}(\mathbb{Z}_n, C_n)$  satisfying  $d'_n(f_n) = d_n \circ f_n = 0$  can be written  $d'_{n+1}(f_{n+1}) = d_{n+1} \circ f_{n+1}$  for some  $f_{n+1} \in \text{Hom}_{\mathbb{Z}}(\mathbb{Z}_n, C_{n+1})$ .

Since  $1 \in \text{Hom}_{\mathbb{Z}}(\mathbb{Z}_n, C_n)$  satisfies

$$d'_n(1(\mathbb{Z}_n)) = d_n(1(\mathbb{Z}_n)) = 0$$

we have, for some  $f \in \text{Hom}_{\mathbb{Z}}(\mathbb{Z}_n, C_n)$   $d_{n+1} \circ f(1(\mathbb{Z}_n)) = 1(\mathbb{Z}_n) = \mathbb{Z}_n$ ,

So  $\text{Im } d_{n+1} = \mathbb{Z}_n$  and so  $H_n(C) = 0$ .

→ Converse: Consider the sequence of  $\mathbb{Z}$  modules

$$\dots \xrightarrow{d} \mathbb{Z}_4 \xrightarrow{d} \mathbb{Z}_4 \xrightarrow{d} \mathbb{Z}_4 \xrightarrow{d} \dots \quad \text{where } d_n(x) = 2x \quad \forall n.$$

For all  $n$ ,  $\mathbb{Z}_n = \langle 2 \rangle = B_n$ , so  $H_n(C) = 0 \quad \forall n$ .

Now, notice  $\text{Hom}_{\mathbb{Z}}(\langle 2 \rangle, \mathbb{Z}_4) = \{0, 1\}$  where 0 is the zero hom. and 1 is inclusion.  $\text{Ker } d'_n = \{0, 1\}$ ,  $\text{Im } d'_{n+1} = \{0\}$ , so

$$H_n(\text{Hom}_{\mathbb{Z}}(\langle 2 \rangle, \mathbb{Z}_4)) \neq 0$$

$$f=0: d \circ f = 0$$

$$f=1: d \circ f = 0$$

$$\begin{array}{ccc} & \langle 2 \rangle & \\ f \swarrow & & \searrow \\ \mathbb{Z}_4 & \xrightarrow{d} & \mathbb{Z}_4 \end{array}$$

$$1(\langle 2 \rangle) = \langle 2 \rangle$$

So converse is not true.

### Exercise 1.1.5:

1)  $\Rightarrow$  2) If  $C$  is exact  $\text{Im}(d_{n+1}) = \text{Ker}(d_n)$ , so

$$H_n(C) = \text{Ker}(d_n) / \text{Im}(d_{n+1}) = 0$$

2)  $\Rightarrow$  3) By def  $H_n(0) = 0 \ \forall n$ , so if  $H_n(C) = 0 \ \forall n$ , The induced map  $H_n(0) \rightarrow H_n(C)$  is an isomorphism  $\forall n$ . So  $0 \rightarrow C$  is a quasi iso.

3)  $\Rightarrow$  1) Since each  $\text{Ker}(d_n) / \text{Im}(d_{n+1}) = H_n(C) \cong 0$ ,  $\text{Ker}(d_n) = \text{Im}(d_{n+1})$  iso  $\forall n$ .

---

### Exercise 1.2.1:

Exercise 1.23: Suppose  $\mathcal{A} = \underline{\text{Ch}}$  and  $f$  a chain map,  $f: B \rightarrow C$ .

(3)

Consider the subcomplex of  $B$ ,  $\text{Ker}(f)$ . By definition  $\iota: \text{Ker}(f) \rightarrow B$  satisfies  $\iota \circ f = 0$ , since for each  $n$ ,  $\iota_n \circ f_n = 0$  as  $\iota_n: \text{Ker}(f_n)$  is a kernel of  $f_n$ . Now suppose  $e: A \rightarrow B$  is another chain map s.t.  $e \circ f = 0$ . Then  $e_n \circ f_n = 0$ . So by universal prop of kernel, there exists  $e'_n: A_n \rightarrow \text{Ker}(f_n)$  s.t.  $e_n = e'_n \circ \iota_n$ . Let  $e'$  be the collection of hom's  $e'_n$ . Then it suffices to show that  $d \cdot e'_n = e'_{n-1} \cdot d'$  for all  $n$ . We already know  $d e_n = e_{n-1} \cdot d'$ , so

$$\begin{array}{ccccc}
 A_n & \xrightarrow{d'} & A_{n-1} & & \\
 \downarrow e_n & \searrow e_n & \downarrow e'_{n-1} & \searrow e_{n-1} & \\
 & B_n & \xrightarrow{d} & B_{n-1} & \\
 \uparrow \iota_n & & \downarrow \iota_{n-1} & & \\
 \text{Ker } f_n & \xrightarrow{d} & \text{Ker } f_{n-1} & & 
 \end{array}$$

$$\begin{aligned}
 d \cdot e_n &= d \cdot \iota_n \cdot e'_n \\
 &= \iota_{n-1} \cdot d' \cdot e'_n \quad \text{and}
 \end{aligned}$$

$$e_n \cdot d' = \iota_{n-1} \cdot e'_{n-1} \cdot d'$$

But since we are in an abelian category ~~every kernel is monic~~,  $\iota_{n-1}$  is a monic, i.e. left cancellable. So  $d e'_n = e'_{n-1} \cdot d'$ , which means  $\text{Ker}(f)$  is a kernel for  $f$ .

$$\begin{array}{ccc}
 A & \xrightarrow{e} & B \\
 \downarrow e' & \nearrow \iota & \downarrow f \\
 \text{Ker } f & & C
 \end{array}$$

Exercise 1.2.4: From Ex 1.2.3  $\text{Ker}(g) = \{\text{Ker}(g_n)\}$  is a Kernel of  $g: B \rightarrow C$ . Similarly  $\text{coker}(f) = \{\text{coker}(f_n)\}$  is a coker. of  $f: A \rightarrow B$ . Now by def  $\text{Im}(f) = \{\text{Ker}(\text{coker } f_n)\}$ .

Then sequence is exact iff,  $\text{Ker}(g) = \text{Im}(f)$ , iff

$\text{Ker}(g_n) = \text{Ker}(\text{coker}(f_n)) = \text{Im}(f_n)$  iff  $A_n \rightarrow B_n \rightarrow C_n$  exact.

Exercise 1.2.5:  $\text{Tot}(C) = \text{Tot}^\pi(C)_n = \prod_{p+q=n} C_{p,q}$

$$d = d^h + d^v \quad d^h: C_{p,q} \rightarrow C_{p-1,q} \quad d^v: C_{p,q} \rightarrow C_{p,q-1}$$

Suppose  $C$  is bounded w/ exact rows. That is each  $\text{Tot}^\pi(C)_n$  is always a finite product.

0  $\xrightarrow{\sigma}$



# Exercise 1.2.7:

$$\dots \rightarrow C_{n+1} \rightarrow C_n \rightarrow C_{n-1} \rightarrow \dots \text{ a complex } \textcircled{4}$$

Let  $Z(C)$  be the complex  $\dots \xrightarrow{0} Z_{n+1}(C) \xrightarrow{0} Z_n(C) \xrightarrow{0} Z_{n-1}(C) \xrightarrow{0} \dots$   
 and  $B(C)$  the complex  $\dots \xrightarrow{0} B_{n+1}(C) \xrightarrow{0} B_n(C) \xrightarrow{0} B_{n-1}(C) \xrightarrow{0} \dots$

Then  $B(C)[-1]$  is the complex  $\dots \rightarrow B_n(C) \rightarrow B_{n-1}(C) \rightarrow B_{n-2}(C) \rightarrow \dots$

So we have

$$\begin{array}{ccccccc} & & \downarrow 0 & & \downarrow & & \downarrow 0 \\ 0 & \rightarrow & Z_{n+1} & \rightarrow & C_{n+1} & \rightarrow & B_n \rightarrow 0 \\ & & \downarrow 0 & & \downarrow d & & \downarrow 0 \\ 0 & \rightarrow & Z_n & \rightarrow & C_n & \rightarrow & B_{n-1} \rightarrow 0 \\ & & \downarrow 0 & & \downarrow d & & \downarrow 0 \\ 0 & \rightarrow & Z_{n-1} & \rightarrow & C_{n-1} & \rightarrow & B_{n-2} \rightarrow 0 \\ & & \downarrow 0 & & \downarrow & & \downarrow 0 \end{array}$$

The rows are exact because  $0 \rightarrow \ker(d_n) \rightarrow C_n \rightarrow \text{im}(d_n) \rightarrow 0$  is always exact. Then by Ex 1.2.4, the chain complex is exact.

ALT: Consider the map  $d: C \rightarrow C[-1]$

$$\begin{array}{ccccccc} \dots \rightarrow C_{n+1} & \xrightarrow{d_{n+1}} & C_n & \xrightarrow{d_n} & C_{n-1} & \rightarrow & \dots \\ & \downarrow d_{n+1} & \downarrow d_n & & \downarrow d_{n-1} & & \\ \dots \rightarrow C_n & \xrightarrow{d_n} & C_{n-1} & \xrightarrow{d_{n-1}} & C_{n-2} & \rightarrow & \dots \end{array}$$

which is certainly a chain map. Now this means  $d_{n-1} \cdot d_n = 0$

Then  $\text{coker } d_n = d_{n-1}$ , so  $\ker(d_{n-1}) = \ker(\text{coker } d_n) = \text{im } d_n$   $\forall n$ .

So  $\ker(d) = \{\ker d_n\} = \{Z_n\}$  and

$\text{coker}(d) = \{d_n\} = \{B_n\}$  so since

$0 \rightarrow \ker(d) \rightarrow C \rightarrow \text{coker}(d) \rightarrow 0$  always exact.

$$0 \rightarrow Z \rightarrow C \rightarrow B(-1) \rightarrow 0$$

Cont:

$$0 \longrightarrow H(C) \longrightarrow C/B(C) \longrightarrow Z(C)[-1] \longrightarrow H(C)[-1] \longrightarrow 0$$

Exercise 1.2.8:  $f: B \rightarrow C$  a morphism

$$\begin{array}{ccccccc} \cdots & \longrightarrow & B_{n+1} & \longrightarrow & B_n & \longrightarrow & B_{n-1} \longrightarrow \cdots \\ & & \downarrow f_{n+1} & & \downarrow f_n & & \downarrow f_{n-1} \\ \cdots & \longrightarrow & C_{n+1} & \longrightarrow & C_n & \longrightarrow & C_{n-1} \longrightarrow \cdots \end{array}$$

we can make  $D$  to be the double complex

$$\begin{array}{ccccccc} & & \downarrow & & \downarrow & & \downarrow \\ \cdots & \longrightarrow & 0 & \xrightarrow{0} & 0 & \xrightarrow{0} & 0 \longrightarrow \cdots \\ & & \downarrow 0 & & \downarrow 0 & & \downarrow 0 \\ \cdots & \longrightarrow & B_{n+1,1} & \longrightarrow & B_{n,1} & \longrightarrow & B_{n-1,1} \longrightarrow \cdots \\ & & \downarrow (-1)^{n+1} f_{n+1} & & \downarrow (-1)^n f_n & & \downarrow (-1)^{n-1} f_{n-1} \\ \cdots & \longrightarrow & C_{n+1,0} & \longrightarrow & C_{n,0} & \longrightarrow & C_{n-1,0} \longrightarrow \cdots \\ & & \downarrow 0 & & \downarrow 0 & & \downarrow 0 \\ \cdots & \longrightarrow & 0 & \xrightarrow{0} & 0 & \xrightarrow{0} & 0 \longrightarrow \cdots \\ & & \downarrow & & \downarrow & & \downarrow \end{array}$$

$B$  and  $C$  can be made to double complexes by making every other row the "0" complex.



(5)

$$0 \rightarrow A \xrightarrow{f} B \xrightarrow{g} C \rightarrow 0 \quad \text{epi iff } g \text{ epi}$$

$$\begin{array}{ccccccc}
 & 0 & & 0 & & 0 & & 0 \\
 & \downarrow & & \downarrow & & \downarrow & & \downarrow \\
 \cdots & \rightarrow & A_{n+1} & \rightarrow & A_n & \xrightarrow{d_{n-1}} & A_{n-1} & \rightarrow & A_{n-2} \\
 & & \downarrow f_{n+1} & & \downarrow f_n & & \downarrow f_{n-1} & & \downarrow f_{n-2} \\
 \cdots & \rightarrow & B_{n+1} & \rightarrow & B_n & \xrightarrow{d_n(b)} & B_{n-1} & \rightarrow & B_{n-2} \\
 & & \downarrow g_{n+1} & & \downarrow g_n & & \downarrow g_{n-1} & & \\
 \cdots & \rightarrow & C_{n+1} & \xrightarrow{d_{n+1}} & C_n & \xrightarrow{d_n} & C_{n-1} & \rightarrow & \cdots \\
 & & \downarrow & & \downarrow & & \downarrow & & \\
 & & 0 & & 0 & & 0 & & 
 \end{array}$$

$\text{im}(f) = \ker(g)$

A, B Exact: WTS  $\ker(d_n) = \text{Im}(d_{n+1})$  (it's a sequence so already have  $\text{Im}(d_{n+1}) \subseteq \ker(d_n)$ )

let  $c \in \ker(d_n)$ ,  $g_n$  surj. so  $\exists b \in B_n$  s.t.  $g_n(b) = c$ .

So  $0 = d_n(c) = d_n(g_n(b)) = g_{n-1}d_n(b)$ , so  $d_n(b) \in \ker g_{n-1} = \text{im } f_{n-1}$

$\exists a \in A_{n-1}$  s.t.  $f_{n-1}(a) = d_n(b)$

Then  $0 = d_{n-1}d_n(b) = d_{n-1}f_{n-1}(a) = f_{n-2}d_{n-1}(a)$

So  $d_{n-1}(a) \in \ker f_{n-2}$ , but  $f_{n-2}$  is injective, so  $d_{n-1}(a) = 0$ .

But  $A$  is exact so  $\exists a' \in A_n$  s.t.  $d_n(a') = a$

So  $f_{n-1}d_n(a') = f_{n-1}(a) = d_n(b)$

$$d_n \cdot f_n(a')$$

$$b - f_n(a')$$

$$d_n(f_n(a') - b) = 0$$

$$f_n(a') - b$$

$$\in \ker d_n = \text{im } d_{n+1} \quad \exists b' \in B_{n+1} \text{ s.t.}$$

$$d_{n+1}(b') = b - f_n(a')$$

$$d_{n+1} \cdot g_{n+1}(b') = g_n(d_{n+1}(b'))$$

$$= g_n(f_n(a') - b)$$

$$= g_n(b) - g_n(f_n(a')) = c$$

So  $c \in \text{im}(d_{n+1})$

$$\begin{array}{ccccccc}
 & 0 & & 0 & & 0 & \\
 & \downarrow & & \downarrow & & \downarrow & \\
 0 & \longrightarrow & A' & \xrightarrow{f} & B' & \xrightarrow{g} & C' \longrightarrow 0 \\
 & & \downarrow c' & & \downarrow k' & & \downarrow l' \\
 0 & \longrightarrow & A & \xrightarrow{d_A} & B & \xrightarrow{d_B} & C \longrightarrow 0 \\
 & & \downarrow e & & \downarrow & & \downarrow \\
 0 & \longrightarrow & A'' & \longrightarrow & B'' & \longrightarrow & C'' \longrightarrow 0 \\
 & & \downarrow & & \downarrow & & \downarrow \\
 & & 0 & & 0 & & 0
 \end{array}$$

all columns exact.

1) Bottom two rows exact

Claim. Top row a complex.  $0 \rightarrow A' \xrightarrow{f} B'$  is zero b/c first map is 0,  
 Similarly w/  $B' \rightarrow C' \rightarrow 0$ . Then we just need to check that  
 $A' \xrightarrow{f} B' \xrightarrow{g} C'$  is the zero map.

$$d_A e'(a) = k' \cdot f(a)$$

$0 = d_B d_A e'(a) = d_B k' f(a) = l' \cdot g \cdot f(a) \Rightarrow g \cdot f(a) \in \text{Ker } l'$   
 But exactness at  $C'$  means  $\text{Ker } l' = \text{im } 0 = 0$ , so  $g \cdot f(a) = 0$   
 and  $g \cdot f = 0$ , so top row is a complex.

Exercise 1.3.1: Let  $0 \rightarrow A \rightarrow B \rightarrow C \rightarrow 0$  be a s.e.s. Suppose two of the three complexes are exact. ⑤

$$\begin{array}{ccccccc}
 & & 0 & & 0 & & 0 \\
 & & \downarrow & & \downarrow & & \downarrow \\
 & & A_n & \longrightarrow & A_{n-1} & \longrightarrow & A_{n-2} \longrightarrow \dots \\
 & & \downarrow & & \downarrow & & \downarrow \\
 \longrightarrow & B_{n+1} & \longrightarrow & B_n & \longrightarrow & B_{n-1} & \longrightarrow B_{n-2} \longrightarrow \dots \\
 & \downarrow & & \downarrow & & \downarrow & \\
 \longrightarrow & C_{n+1} & \longrightarrow & C_n & \longrightarrow & C_{n-1} & \longrightarrow \dots \\
 & \downarrow & & \downarrow & & \downarrow & \\
 & & & 0 & & 0 & 
 \end{array}$$

### Exercise 1.3.2:



Exercise 1.3.3:

(6)

$$\begin{array}{ccccccccc} A' & \longrightarrow & B' & \longrightarrow & C' & \longrightarrow & D' & \longrightarrow & E' \\ \downarrow a & & \downarrow b & & \downarrow c & & \downarrow d & & \downarrow e \\ A & \longrightarrow & B & \longrightarrow & C & \longrightarrow & D & \longrightarrow & E \end{array}$$

1) Suppose  $b, d$  are monic and  $a$  is epi



Exercise 13.4: Consider  $0 \rightarrow Z \xrightarrow{\iota} C \xrightarrow{\varphi} B(-1) \rightarrow 0$ . ②

$$\rightarrow H_{n+1}(B(-1)) \xrightarrow{\beta} H_n(\mathbb{Z}) \rightarrow H_n(C) \rightarrow H_n(B(-1)) \rightarrow H_{n-1}(\mathbb{Z}) \rightarrow \dots$$

\* Rows of bicomplex exact, but columns aren't. Homologies are col's

$$H_n(z) = z_n / 0 = z_n$$

$$\cdots \rightarrow B_n \xrightarrow{\partial_n} B_{n-1} \xrightarrow{\partial_{n-1}} B_{n-2} \rightarrow \cdots$$

$$H_n(B(-1)) = B_{n-1}/0 = B_{n-1}$$

50

factor through 0

$$\begin{array}{ccccccc} \rightarrow B_{n+1} & \hookrightarrow & Z_{n+1} & \xrightarrow{\quad \tilde{\tau} \quad} & H_{n+1}(C) & \xrightarrow{\quad 0 \quad} & B_{n+1} \hookrightarrow Z_n \xrightarrow{\quad \tau \quad} H_n(C) \xrightarrow{\quad 0 \quad} B_{n-1} \hookrightarrow Z_{n-1} \xrightarrow{\quad \tau \quad} H_{n-1}(C) \xrightarrow{\quad 0 \quad} B_{n-2} \hookrightarrow Z_{n-2} \rightarrow \dots \\ & & & & \parallel & & \\ & & & & Z_{n+1}/B_{n+1} & & \end{array}$$

So

$$\begin{array}{ccccccc} \cdots & \rightarrow & 0 & \rightarrow & B_{n+1} & \hookrightarrow & Z_{n+1} \rightarrow H_{n+1}(C) \rightarrow 0 \\ & & & & & & \searrow \\ & & & & & & B_n \hookrightarrow Z_n \rightarrow H_n(C) \rightarrow 0 \\ & & & & & & \searrow \\ & & & & & & B_{n-1} \hookrightarrow Z_{n-1} \rightarrow H_{n-1}(C) \rightarrow 0 \dots \end{array}$$

1.3.5: Take  $0 \rightarrow \ker f \rightarrow C \rightarrow \operatorname{im} f \rightarrow 0$

$$0 \rightarrow \text{im } f \rightarrow D \rightarrow \text{Coker } f \rightarrow 0$$

Take long exact seq. in homology for  $\mathcal{E}_n C \cong \mathcal{E}_n \text{im} f \cong \mathcal{E}_n D$ .

Exercise 1.3.5: Suppose  $f: C. \rightarrow D.$  is a chain map. Suppose  $\text{Ker}(f)$  and  $\text{coker}(f)$  are acyclic. Then we have the seq. of chain maps

$$\text{Ker}(f) \rightarrow C. \xrightarrow{f} D. \rightarrow \text{Coker}(f)$$

So by exercise 1.1.2 there is an induced seq on homology

$$H_n(\text{Ker}(f)) \rightarrow H_n(C) \rightarrow H_n(D) \rightarrow H_n(\text{Coker}(f))$$

But since  $\text{Ker } f, \text{coker } f$  acyclic, the two ends are 0, so

$H_n(C) \cong H_n(D)$ , which means  $C. \rightarrow D.$  is a quasi-iso.

Converse: Let  $C.$  be the seq.  $\dots \rightarrow C^2 \rightarrow C^2 \rightarrow C^2 \rightarrow \dots$

where  $f_n(a,b) = (b,0)$ . Let  $D.$  be the sequence

$$\dots \rightarrow C^3 \xrightarrow{g} C^3 \xrightarrow{g} C^3 \rightarrow \dots \text{ where } g_n(a,b,c) = (0,c,0).$$

Finally define  $h: C^2 \rightarrow C^3$  by  $h(a,b) = (0,a,b)$ . Then both

$C$  and  $D$  are complexes with  $Z_n(C) \cong C^2$ ,  $B_n(C) \cong C$  and

$$Z_n(D) \cong C, B_n(D) \cong C$$

Converse:

$$C: \dots \rightarrow C \xrightarrow{f} C \xrightarrow{f} C \rightarrow \dots \quad f_n(a) = 0$$

$$D: \dots \rightarrow C^3 \xrightarrow{g} C^3 \xrightarrow{g} C^3 \rightarrow \dots \quad g_n(a,b,c) = (c,0,0)$$

$$Z_n(C) = C, B_n(C) = 0$$

$$Z_n(D) = \{(a,b,0)\}, B_n(D) = \{(a,0,0)\}$$

$$h: C \rightarrow D \quad h(a) = (0,a,0) \quad H_n(C) \cong C \cong H_n(D)$$

$$\text{Ker } h = 0 \quad \text{coker } h = \{(a,0,c)\} \quad h^2(a,0,c) = (c,0,0)$$

$$\dots \rightarrow 0 \rightarrow 0 \rightarrow \mathbb{Z} \rightarrow \mathbb{Z} \rightarrow 0 \rightarrow \dots$$

$$\downarrow 0 \quad \downarrow \text{id} \quad \downarrow 0$$

quasi iso.

$$\dots \rightarrow 0 \rightarrow \mathbb{Z} \rightarrow \mathbb{Z} \rightarrow 0 \rightarrow 0 \rightarrow \dots$$

$$\text{Ker } 0 \rightarrow 0 \rightarrow 0 \rightarrow \mathbb{Z} \rightarrow 0$$

$$\text{coker } 0 \rightarrow \mathbb{Z} \rightarrow 0 \rightarrow 0 \rightarrow 0$$

Nontrivial

### Exercise 1.4.2:

$\Rightarrow$ )  $C$  split, then there exist maps  $S_n: C_n \rightarrow C_{n+1}$  s.t.  $d = dSd$ .

Consider the S.E.S.  $0 \rightarrow Z_n \hookrightarrow C_n \xrightarrow{d} \text{im } d_n \rightarrow 0$ . It suffices to show this is a split exact sequence.

Then if  $b \in \text{Im } d_n$ ,  $dS_n(\underset{\text{ind}}{b}) = dSd(a) = d(a) = b$  for some  $a \in C_n$ .

So  $S_n$  is a splitting map for the S.E.S. and so

$$C_n \cong Z_n \oplus \text{im } d_n \cong Z_n \oplus C_n / Z_n$$

Now, consider the seq.  $0 \rightarrow \text{Ker } dS \hookrightarrow Z_n \xrightarrow{dS} B_n \rightarrow 0$

we have the natural inclusion  $\iota: B_n \rightarrow Z_n$ , so for any  $b \in$

$$\text{Im } d_{n+1} = B_n, \quad dS|_{B_n} \circ \iota(b) = dS|_{Z_n}(b) = dSd(a) = d(a) = b$$

for some  $a \in C_{n+1}$ . So  $\iota$  is a splitting map and  $Z_n \cong B_n \oplus \text{Ker } dS$ .

Then writing  $0 \rightarrow B_n \hookrightarrow Z_n \xrightarrow{\nu} \text{Ker } dS \rightarrow 0$  is a S.E.S.

where  $\nu: Z_n \rightarrow \text{Ker } dS$  is the proj., shows  $\text{Ker } dS \cong Z_n / B_n$ .

$\Leftarrow$ ) Now suppose  $C_n \cong Z_n \oplus B'_n$  and  $Z_n \cong B_n \oplus H'_n$ . We have the

S.E.S.  $0 \rightarrow Z_n \hookrightarrow C_n \xrightarrow{d} B'_n \rightarrow 0$ . Since there is a natural

in

Exercise 1.4.1: Suppose  $C$  is an acyclic and bounded below, complex of free  $R$ -modules.  $C$  is already acyclic so suffices to show it is split.

### Exercise 1.4.3:

$\Rightarrow$ ) Suppose  $C$  is split exact.

Then there exists  $S_n: C_n \rightarrow C_{n+1}$

s.t.  $d = dSd$ .

$$\begin{array}{ccccccc} \cdots & \rightarrow & C_{n+1} & \xrightarrow{d} & C_n & \rightarrow & C_{n-1} \rightarrow \cdots \\ & & \downarrow \mathbb{1} & \swarrow S_n & \downarrow \mathbb{1} & \swarrow S_{n-1} & \downarrow \mathbb{1} \\ \cdots & \rightarrow & C_{n+1} & \xrightarrow{d} & C_n & \rightarrow & C_{n-1} \rightarrow \cdots \end{array}$$

Then from ex 1.4.2 we know

$$C_n \cong B_n \oplus B_{n-1} \text{ for all } n.$$





Exercise 1.5.1: By ex. 1.4.3 it suffices to show that

$\text{id}_{\text{cone}(c)}$  is nullhomotopic, w/  $\text{id}_{\text{cone}(c)} = ds + sd$ .  $s(c', c) = (-c, 0)$

$$\begin{array}{ccccccc} \cdots & \longrightarrow & C_n \oplus C_{n+1} & \longrightarrow & C_{n-1} \oplus C_n & \longrightarrow & C_{n-2} \oplus C_{n-1} \longrightarrow \cdots \\ & & \downarrow \text{id} & \swarrow s_n & \downarrow \text{id} & \swarrow s_{n-1} & \downarrow \text{id} \\ \cdots & \longrightarrow & C_n \oplus C_{n+1} & \longrightarrow & C_{n-1} \oplus C_n & \longrightarrow & C_{n-2} \oplus C_{n-1} \longrightarrow \cdots \end{array}$$

$$\begin{aligned} \text{Then } ds(c', c) &= d(-c, 0) = (-d(-c), d(0) - \text{id}(-c)) \\ &= (d(c), c) \end{aligned}$$

$$\begin{aligned} sd(c', c) &= s(-d(c'), d(c) - c') \\ &= (c' - d(c), 0) \end{aligned}$$

$$\text{So } (sd + ds)(c', c) = (c', c) = \text{id}_{\text{cone}(c)}(c', c).$$

Exercise 1.5.2:

$\Rightarrow$ ) Suppose  $f$  null-homotopic,  $\exists S_n: C_n \rightarrow D_{n+1}$  s.t.  $f = sd + ds$

Let  $g = -s + f: \text{Cone}(c) \rightarrow D$ . Suffices to check  $gd = dg$ .

$$gd(c', c) = g(d(c'), d(c) - c')$$

$$= -s(-d(c')) + f(d(c) - c')$$

$$= \cancel{sd(c')} + (sd + ds)d(c) - \cancel{sd(c')} - ds(c')$$

$$= dsd(c) - ds(c')$$

$$dg(c', c) = d(-s(c') + f(c))$$

$$= d(-s(c')) + d(\cancel{ds} + sd)(c)$$

$$= -ds(c') + dsd(c)$$

$$\begin{aligned} g(c', c) &= g(c', 0) + g(0, c) \\ &= -s(c', 0) + f(0, c) \\ &= -s(c') + f(c). \end{aligned}$$

So  $g$  is a chain map.

$\Leftarrow$ ) Suppose  $f$  extends to  $g = -s + f$ . Then  $gd = dg$  or

$$sd(c') + \cancel{fd(c)} - f(c') = -ds(c') + d\cancel{f(c)}$$

$$\Leftrightarrow f(c') = (sd + ds)c', \text{ Thus } f \text{ is null homotopic.}$$

### Exercise 1.5.3:

$\Rightarrow$ ) Suppose  $f, g: C \rightarrow D$  chain homotopic,  $f - g = ds + sd$  or  $f = ds + sd + g$ .  
Then  $h = f + s + g: \text{Cyl}(C) \rightarrow D$  and

$$\begin{aligned} dh(c_1, c', c_2) &= df(c_1) + ds(c') + dg(c_2) \\ &= d(\cancel{ds} + sd + g)(c_1) + ds(c') + dg(c_2) \\ &= dsd(c_1) + dg(c_1) + ds(c') + dg(c_2) \end{aligned}$$

$$\begin{aligned} hd(c_1, c', c_2) &= h(d(c_1) + c', -d(c'), d(c_2) - c') \\ &= fd(c_1) + f(c') + s(-d(c')) + gd(c_2) - g(c') \\ &= (ds + \cancel{sd} + g)d(c_1) + (ds + \cancel{sd} + g)(c') - \cancel{sd(c')} + gd(c_2) - \cancel{g(c')} \\ &= dsd(c_1) + gd(c_1) + ds(c') + gd(c_2) \end{aligned}$$

So  $h$  is a chain map.

$\Leftarrow$ ) Suppose  $h = f + s + g: \text{Cyl}(C) \rightarrow D$  is a chain map.

Then  $hd = dh$  and

$$\begin{aligned} dh(c_1, c', c_2) &= d\cancel{f(c_1)} + ds(c') + d\cancel{g(c_2)} \\ - hd(c_1, c', c_2) &= \cancel{fd(c_1)} + f(c') - \cancel{sd(c')} + \cancel{gd(c_2)} - g(c') \end{aligned}$$

$$0 = ds(c') + sd(c') + g(c') - f(c')$$

$$\Leftrightarrow f(c') - g(c') = (ds + sd)(c')$$

So  $f, g$  are homotopic.

# Exercise 2.2.1:

$\Rightarrow$  Suppose  $P$  is a projective in  $\text{Ch } A$

Then if  $f: D \rightarrow C$  is a surj. chain map

and  $\gamma: P \rightarrow C$  is a chain map, there exists a chain map  $\beta: P \rightarrow D$

s.t.  $f \circ \beta = \gamma$ . Now, this means for each  $n$ , each  $f_n$  is a surj.

where  $f_n \circ \beta_n = \gamma_n$  which means each  $P_n$  is projective.

$$\begin{array}{ccc} & & P \\ & \swarrow \gamma & \downarrow \gamma \\ B & \cdots & \\ & \searrow & \\ D & \xrightarrow{f} & C \end{array}$$

$$\begin{array}{ccccccc} \cdots & \rightarrow & P_{n+1} & \xrightarrow{\gamma_{n+1}} & P_n & \xrightarrow{\gamma_n} & P_{n-1} \rightarrow \cdots \\ & & \searrow & & \searrow & & \searrow \\ & & C_{n+1} & \xrightarrow{\gamma_n} & C_n & \xrightarrow{\gamma_{n-1}} & C_{n-1} \rightarrow \cdots \\ & \swarrow & \uparrow & \swarrow & \uparrow & \swarrow & \uparrow \\ \cdots & \rightarrow & D_{n+1} & \xrightarrow{f_{n+1}} & D_n & \xrightarrow{f_n} & D_{n-1} \rightarrow \cdots \end{array}$$

$$\begin{array}{ccc} & & P[-1] \\ & \swarrow & \downarrow \text{id} \\ \text{Cone}(P) & \xrightarrow{d} & P[-1] \end{array}$$

Recall the S.E.S.  $0 \rightarrow P \xrightarrow{\iota} \text{Cone}(P) \xrightarrow{d} P[-1] \rightarrow 0$

Since  $P$  is projective, if  $\exists \alpha: P[-1] \rightarrow C$  w/  $g: D \rightarrow C$  surj.

we can choose  $\beta: P[-1] \rightarrow D$  by taking the collection of maps from each  $P_n$  (since each  $P_n$  is proj), so  $P[-1]$  is also proj. Then we get

This means there exists a splitting map  $\beta: P[-1] \rightarrow \text{Cone}(P)$

s.t.  $d \circ \beta = \text{id}$ . We also have  $\pi: \text{Cone}(P) \rightarrow P$  the collection of projections, which will also be a splitting map.

~~(the S.E.S. as a chain complex of chain complexes, it is split exact. So  $\text{Cone}(P) \cong P \oplus P[-1]$ .)~~

Then it is a split exact sequence and we have that

the identity on this complex is null homotopic (Ex 1.4.3).

Moreover this means  $H_n(C) \xrightarrow{\text{id}_g} H_n(C)$  is the zero map, but is also an isomorphism since it's the induced map by the identity.

$$\begin{array}{ccccc} & & (b, c) \mapsto (d(b), d(c) - \beta(b)) & & \\ P_n & \rightarrow & P_n \oplus P_{n-1} & \rightarrow & P_{n-1} \\ & & \downarrow & & \\ & & P_{n-1} \oplus P_{n-2} & & \end{array}$$

## Exercise 2.2.2:

$$0 \rightarrow A \xrightarrow{\varphi} B \xrightarrow{\psi} C \rightarrow 0$$

WTS

$$0 \rightarrow \text{Hom}(M, A) \xrightarrow{\varphi_*} \text{Hom}(M, B) \xrightarrow{\psi_*} \text{Hom}(M, C)$$

$$\begin{array}{ccc} & M & \\ \gamma \swarrow & & \downarrow \varphi_* \gamma \\ A & \xrightarrow{\varphi} & B \end{array}$$

Suppose  $\varphi_* \gamma = 0$ . Since  $\varphi$  injective  $\gamma = 0$ , so  $\varphi_*$  is injective.

$$\varphi_* \gamma = \varphi \circ \gamma$$

$$\begin{array}{ccc} & M & \\ \gamma \swarrow & & \downarrow \varphi_* \gamma \\ B & \xrightarrow{\varphi} & C \end{array}$$

Let  $\gamma \in \text{Hom}(M, A)$ . Then  $\psi_* \varphi_* \gamma = \psi \circ \varphi \circ \gamma = 0 \circ \gamma = 0$ .

So  $\text{im } \varphi_* \subseteq \text{Ker } \psi_*$

Let  $\beta \in \text{Hom}(M, B)$  s.t.  $\psi_* \beta = 0$ .

Need  $\gamma \in \text{Hom}(M, A)$  s.t.  $\varphi_* \gamma = \beta = \varphi \circ \gamma$

Then  $\text{im } \beta \subseteq \text{Ker } \psi = \text{im } \varphi$  i.e.  $A \xrightarrow{\varphi} \text{im } \beta$

~~for each~~

So for each  $\beta(m) \in \text{im } \beta$ ,  $\exists a_m \in A$  s.t.  $\varphi(a_m) = \beta(m)$

define  $f: M \rightarrow A$  by  $f(m) = a_m$

So  $\varphi(f(m)) = \varphi(a_m) = \beta(m)$

$$\begin{array}{ccc} & M & \\ f \swarrow & & \downarrow \beta \\ A & \xrightarrow{\varphi} & B \end{array} \quad \begin{array}{c} \searrow \psi \\ C \end{array}$$



Exercise 2.2.3: Let  $\dots \rightarrow P_2 \rightarrow P_1 \rightarrow P_0 \rightarrow 0$  be a complex of projectives

=> 1) Suppose  $\varepsilon: P_2 \rightarrow M$  gives a resolution for  $M$ .

$$\begin{array}{ccccccc} \dots & \rightarrow & P_2 & \rightarrow & P_1 & \rightarrow & P_0 \rightarrow 0 \rightarrow \dots \\ & & \downarrow & & \downarrow & & \downarrow \varepsilon \\ \dots & \rightarrow & 0 & \rightarrow & 0 & \rightarrow & M \rightarrow 0 \rightarrow \dots \\ & & & & & & \downarrow \\ & & & & & & 0 \end{array}$$

Since  $\varepsilon: P \rightarrow M$  a resolution we have exactness at each  $P_i$

So  $H_i(P_i) = 0 \quad \forall i \geq 0$ . Since there is also exactness at  $M$

$\varepsilon_*: H_0(P_0) \cong H_0(M) = 0$ , so this is a quasi-iso

<=> Now suppose we have a quasi iso as above. Then

$H_i(P_i) = 0 \quad \forall i \geq 0$  and  $\varepsilon_*: H_0(P_0) \cong H_0(M)$  implies exactness at  $M$ , so

$$\dots \rightarrow P_2 \rightarrow P_1 \rightarrow P_0 \xrightarrow{\varepsilon} M \rightarrow 0 \rightarrow \dots$$

is all exact and so is a proj. res.

→ Or just use something like Ex 1.1.5.

